List, Ascii, String, and Option serializers done.

lib/Combinators.v
@@ -2,6 +2,54 @@ Require Import StructTactics.
 Require Import List.
 Require Import Types.
 
+Definition option_serialize
+           {T: Type}
+           {tSerializer: Serializer T}
+           (o: option T) :=
+  match o with
+    | None => serialize false
+    | Some t => serialize true ++ serialize t
+  end.
+
+Definition option_deserialize
+           {T: Type}
+           {tSerializer: Serializer T}
+           (bin: list bool) : option (option T * list bool) :=
+  match deserialize bin with
+  | None => None
+  | Some (b, rest) =>
+  match b with
+  | false => Some (None, rest)
+  | true =>
+  match deserialize rest with
+  | None => None
+  | Some (t, rest) =>
+    Some (Some t, rest)
+  end
+  end
+  end.
+
+Lemma option_serialize_reversible :
+  forall {T: Type}
+    {tSerializer: Serializer T}
+    (o: option T) (bin: list bool),
+    option_deserialize (option_serialize o ++ bin) = Some (o, bin).
+Proof.
+  unfold option_deserialize, option_serialize.
+  intros T tSerializer o bin.
+  destruct o; simpl; auto.
+  now rewrite Serialize_reversible.
+Qed.
+
+Instance Option_Serializer :
+  forall (T: Type)
+    {tSerializer: Serializer T}, Serializer (option T) :=
+  {
+    serialize := option_serialize;
+    deserialize := option_deserialize;
+    Serialize_reversible := option_serialize_reversible
+  }.
+
 Definition pair_serialize
            {A B: Type}
            {aSerializer: Serializer A}
@@ -16,40 +64,162 @@ Definition pair_deserialize
            {bSerializer: Serializer B}
            (bin: list bool) : option ((A * B) * list bool) :=
   match deserialize bin with
+  | None => None
+  | Some (a, rest) =>
+  match deserialize rest with
+  | None => None
+  | Some (b, remainder) =>
+    Some ((a, b), remainder)
+  end
+  end.
+
+Lemma pair_serialize_reversible :
+  forall {A B: Type}
+    {aSerializer: Serializer A}
+    {bSerializer: Serializer B}
+    (p: A * B) (bin: list bool),
+    pair_deserialize (pair_serialize p ++ bin) = Some (p, bin).
+Proof.
+  intros.
+  unfold pair_serialize.
+  break_match.
+  unfold pair_deserialize.
+  rewrite app_assoc_reverse.
+  now repeat rewrite Serialize_reversible.
+Qed.
+
+Instance Pair_Serializer :
+  forall (A B: Type)
+    {aSerializer: Serializer A}
+    {bSerializer: Serializer B}, Serializer (A * B) :=
+  {
+    serialize := pair_serialize;
+    deserialize := pair_deserialize;
+    Serialize_reversible := pair_serialize_reversible
+  }.
+
+Definition triple_serialize
+           {A B C: Type}
+           {aSerializer: Serializer A}
+           {bSerializer: Serializer B}
+           {cSerializer: Serializer C}
+           (t: A*B*C) :=
+  let (p, c) := t in
+  let (a, b) := p in
+  (serialize a) ++ (serialize b) ++ (serialize c).
+
+Definition triple_deserialize
+           {A B C: Type}
+           {aSerializer: Serializer A}
+           {bSerializer: Serializer B}
+           {cSerializer: Serializer C}
+           (bin: list bool): option ((A*B*C) * list bool) :=
+  match deserialize bin with
     | None => None
     | Some (a, rest) =>
   match deserialize rest with
     | None => None
-    | Some (b, remainder) =>
-      Some ((a, b), remainder)
+    | Some (b, rest) =>
+  match deserialize rest with
+    | None => None
+    | Some (c, remainder) =>
+      Some ((a, b, c), remainder)
+  end
   end
   end.
 
-Instance Pair_Serializer : forall (A B : Type), Serializer A -> Serializer B -> Serializer (A * B) :=
+Lemma triple_serialize_reversible :
+  forall {A B C: Type}
+    {aSerializer: Serializer A}
+    {bSerializer: Serializer B}
+    {cSerializer: Serializer C}
+    (t: A * B * C) (bin: list bool),
+    triple_deserialize (triple_serialize t ++ bin) = Some (t, bin).
+Proof.
+  intros.
+  unfold triple_serialize.
+  repeat break_match.
+  unfold triple_deserialize.
+  repeat rewrite app_assoc_reverse.
+  now repeat rewrite Serialize_reversible.
+Qed.
+
+Instance Triple_Serializer :
+  forall (A B C: Type)
+    {aSerializer: Serializer A}
+    {bSerializer: Serializer B}
+    {cSerializer: Serializer C}, Serializer (A * B * C) :=
   {
-    serialize := pair_serialize;
-    deserialize := pair_deserialize;
+    serialize := triple_serialize;
+    deserialize := triple_deserialize;
+    Serialize_reversible := triple_serialize_reversible
   }.
 
+Fixpoint list_serialize_rec
+         {T: Type}
+         {tSerializer: Serializer T}
+         (ts: list T) := 
+  match ts with
+    | nil => nil
+    | hd :: ts => (serialize hd) ++ (list_serialize_rec ts)
+  end.
 
-(* Check pair_deserialize. *)
+Definition list_serialize
+           {T: Type}
+           {tSerializer: Serializer T}
+           (ts: list T) :=
+  nat_serialize (length ts) ++ (list_serialize_rec ts).
 
-(* Lemma pair_serialize_reversible: forall {A B: Type} *)
-(*                                    {aSerializer: Serializer A} *)
-(*                                    {bSerializer: Serializer B} *)
-(*                                    (x: (A * B)) *)
-(*                                    (bin: list bool), *)
-(*                                    pair_deserialize ((pair_serialize x) ++ bin) = Some (x, bin). *)
-(*   intros. *)
-(*   destruct aSerializer. *)
-(*   destruct bSerializer. *)
-(*   unfold pair_serialize. *)
-(*   break_match. *)
-(*   unfold pair_deserialize. *)
-(*   rewrite app_assoc_reverse. *)
-(*   unfold Types.serialize. *)
-(*   unfold Types.deserialize. *)
-(*   rewrite Serialize_reversible. *)
-(*   rewrite Serialize_reversible0. *)
-(*   reflexivity. *)
-(* Qed. *)
+Fixpoint list_deserialize_rec
+         {T: Type}
+         {tSerializer: Serializer T}
+         (count: nat) (bin: list bool) :=
+  match count with
+    | 0 => Some (nil, bin)
+    | S n =>
+  match deserialize bin with
+    | None => None
+    | Some (t, rest) =>
+  match list_deserialize_rec n rest with
+    | None => None
+    | Some (elements, rest) => Some ((t :: elements), rest)
+  end
+  end
+  end.
+
+Definition list_deserialize
+           {T: Type}
+           {tSerializer: Serializer T}
+           (bin: list bool) : option (list T * list bool) :=
+  match nat_deserialize bin with
+    | None => None
+    | Some (count, rest) =>
+      list_deserialize_rec count rest
+  end.
+
+Lemma list_serialize_reversible :
+  forall {T: Type}
+    {tSerializer: Serializer T}
+    (ts: list T) (bin: list bool),
+    list_deserialize (list_serialize ts ++ bin) = Some (ts, bin).
+Proof.
+  unfold list_deserialize, list_serialize.
+  intros T tSerializer ts bin.
+  rewrite app_assoc_reverse.
+  rewrite nat_serialize_reversible.
+  induction ts; auto.
+  simpl.
+  rewrite app_assoc_reverse.
+  rewrite Serialize_reversible.
+  now rewrite IHts.
+Qed.
+
+Instance List_Serializer :
+  forall (T: Type)
+    {tSerializer: Serializer T},
+    Serializer (list T) :=
+  {
+    serialize := list_serialize;
+    deserialize := list_deserialize;
+    Serialize_reversible := list_serialize_reversible
+  }.
