lib/ComplexSerializers.v
@@ -1,0 +1,42 @@
+Require Import Ascii.
+Require Import String.
+Require Import List.
+Require Import Types.
+Require Import Combinators.
+
+Fixpoint string_to_list s :=
+  match s with
+    | EmptyString => nil
+    | String c s' => c :: (string_to_list s')
+  end.
+
+Fixpoint list_to_string l :=
+  match l with
+    | nil => EmptyString
+    | h::l' => String h (list_to_string l')
+  end.
+
+Lemma string_to_list_to_string : forall s,
+                                  list_to_string (string_to_list s) = s.
+Proof.
+  induction s; auto; simpl.
+  now rewrite IHs.
+Qed.
+
+Definition string_serialize (s : string) :=
+  serialize (string_to_list s).
+
+Definition string_deserialize bin : option (string * list bool) :=
+  match deserialize bin with
+    | None => None
+    | Some (cs, rest) => Some (list_to_string cs, rest)
+  end.
+
+Lemma string_serialize_reversible : forall s bin,
+    string_deserialize (string_serialize s ++ bin) = Some (s, bin).
+Proof.
+  unfold string_deserialize, string_serialize.
+  intros s bin.
+  rewrite Serialize_reversible.
+  now rewrite string_to_list_to_string.
+Qed.
